\section{Introduction \& Background}

Hamiltonian 

\begin{equation}
	H = - \frac{1}{2} \sum_{j,k}^{N} J_{jk} \mathbf{S}_j \cdot \mathbf{S}_k - d_z \sum_{j=1}^{N} (S_{j,z})^2 - \mu \sum_{j=1}^{N} \mathbf{B}_j \cdot \mathbf{S}_j 
\end{equation}

Landau-Lifshitz-Gilbert equation 

\begin{align}
	\pd{\mathbf{S}_j}{t} &= \frac{-\gamma}{\mu(1 + \alpha^2)} \left[ \mathbf{S}_j \times \mathbf{H}_j + \alpha \mathbf{S}_j \times (\mathbf{S}_j + \mathbf{H}_j) \right] \\
	\mathbf{H}_j &= -\pd{H}{\mathbf{S}_j} + \boldsymbol{\xi}_j
\end{align}